<?xml version="1.0"?>
<rdf:RDF xmlns="http://www.semanticweb.org/activage/ontologies/2018/4/activage-core#"
     xml:base="http://www.semanticweb.org/activage/ontologies/2018/4/activage-core"
     xmlns:schema="http://schema.org/"
     xmlns:qu="http://purl.org/NET/ssnx/qu/qu#"
     xmlns:ns="http://www.w3.org/2003/06/sw-vocab-status/ns#"
     xmlns:owl="http://www.w3.org/2002/07/owl#"
     xmlns:xsd="http://www.w3.org/2001/XMLSchema#"
     xmlns:skos="http://www.w3.org/2004/02/skos/core#"
     xmlns:rdfs="http://www.w3.org/2000/01/rdf-schema#"
     xmlns:relaSci="http://sweet.jpl.nasa.gov/2.3/relaSci.owl#"
     xmlns:relaMath="http://sweet.jpl.nasa.gov/2.3/relaMath.owl#"
     xmlns:rdf="http://www.w3.org/1999/02/22-rdf-syntax-ns#"
     xmlns:terms="http://purl.org/dc/terms/"
     xmlns:xml="http://www.w3.org/XML/1998/namespace"
     xmlns:fiesta="http://ontology.fiesta-iot.eu/ontologyDocs/fiesta-iot.owl#"
     xmlns:vann="http://purl.org/vocab/vann/"
     xmlns:foaf="http://xmlns.com/foaf/0.1/"
     xmlns:dc="http://purl.org/dc/elements/1.1/">
    <owl:Ontology rdf:about="http://www.semanticweb.org/activage/ontologies/2018/4/activage-core">
        <owl:imports rdf:resource="http://srvgal106.deri.ie:8013/ontology/GOIoTPex.owl"/>
        <owl:imports rdf:resource="http://srvgal106.deri.ie:8013/ontology/GOIoTP.owl"/>
        <rdfs:comment rdf:datatype="http://www.w3.org/2001/XMLSchema#string">ACTIVAGE Ontology: shell classes</rdfs:comment>
        <terms:rights rdf:datatype="http://www.w3.org/2001/XMLSchema#string">This ontology is distributed under a Creative Commons Attribution License - http://creativecommons.org/licenses/by/3.0</terms:rights>
        <dc:title rdf:datatype="http://www.w3.org/2001/XMLSchema#string">ACTIVAGE Ontology</dc:title>
        <dc:description rdf:datatype="http://www.w3.org/2001/XMLSchema#string">ACTIVAGE is a multi-centric Large Scale Pilot Project which aims to build the first interoperable and open AHA-IoT Ecosystem which enables the deployment and operation of Active &amp; Healthy Ageing IoT-based solutions and services in Europe.</dc:description>
    </owl:Ontology>
    


    <!-- 
    ///////////////////////////////////////////////////////////////////////////////////////
    //
    // Annotation properties
    //
    ///////////////////////////////////////////////////////////////////////////////////////
     -->

    


    <!-- http://purl.org/dc/elements/1.1/title -->

    <owl:AnnotationProperty rdf:about="http://purl.org/dc/elements/1.1/title"/>
    


    <!-- 
    ///////////////////////////////////////////////////////////////////////////////////////
    //
    // Classes
    //
    ///////////////////////////////////////////////////////////////////////////////////////
     -->

    


    <!-- http://www.semanticweb.org/activage/ontologies/2018/4/activage-core#AAL -->

    <owl:Class rdf:about="http://www.semanticweb.org/activage/ontologies/2018/4/activage-core#AAL">
        <rdfs:subClassOf rdf:resource="http://inter-iot.eu/GOIoTP#DomainOfInterest"/>
        <rdfs:label xml:lang="en">Ambient Assisted Living</rdfs:label>
    </owl:Class>
    


    <!-- http://www.semanticweb.org/activage/ontologies/2018/4/activage-core#AirTemperatureSensor -->

    <owl:Class rdf:about="http://www.semanticweb.org/activage/ontologies/2018/4/activage-core#AirTemperatureSensor">
        <rdfs:subClassOf rdf:resource="http://www.semanticweb.org/activage/ontologies/2018/4/activage-core#TemperatureSensor"/>
        <rdfs:comment xml:lang="en">Air temperature sensor is a the bulk temperature of the air, not the surface (skin) temperature..</rdfs:comment>
        <rdfs:label xml:lang="en">Air Temperature Sensor</rdfs:label>
    </owl:Class>
    


    <!-- http://www.semanticweb.org/activage/ontologies/2018/4/activage-core#BoardTemperatureSensor -->

    <owl:Class rdf:about="http://www.semanticweb.org/activage/ontologies/2018/4/activage-core#BoardTemperatureSensor">
        <rdfs:subClassOf rdf:resource="http://www.semanticweb.org/activage/ontologies/2018/4/activage-core#TemperatureSensor"/>
        <rdfs:comment xml:lang="en">Board Temperature Sensor ia a sensor that can be used to measure temperature in the board.</rdfs:comment>
        <rdfs:label xml:lang="en">Board Temperature Sensor</rdfs:label>
    </owl:Class>
    


    <!-- http://www.semanticweb.org/activage/ontologies/2018/4/activage-core#City -->

    <owl:Class rdf:about="http://www.semanticweb.org/activage/ontologies/2018/4/activage-core#City">
        <rdfs:subClassOf rdf:resource="http://inter-iot.eu/GOIoTP#DomainOfInterest"/>
        <rdfs:comment xml:lang="en">Smart City as an Internet of Things (IoT) applicative domain.</rdfs:comment>
        <rdfs:label xml:lang="en">Smart City DOI</rdfs:label>
    </owl:Class>
    


    <!-- http://www.semanticweb.org/activage/ontologies/2018/4/activage-core#Decibel -->

    <owl:Class rdf:about="http://www.semanticweb.org/activage/ontologies/2018/4/activage-core#Decibel">
        <rdfs:subClassOf rdf:resource="http://sweet.jpl.nasa.gov/2.3/reprSciUnits.owl#Unit"/>
        <rdfs:comment xml:lang="en">Decibel is a logarithmic unit used to express the ratio of two values of a physical quantity. It is often used to measure sound level.</rdfs:comment>
        <rdfs:label xml:lang="en">Decibel (dB)</rdfs:label>
        <rdfs:seeAlso xml:lang="en">http://www.qudt.org/qudt/owl/1.0.0/unit/Instances.html#Decibel</rdfs:seeAlso>
    </owl:Class>
    


    <!-- http://www.semanticweb.org/activage/ontologies/2018/4/activage-core#DeltaDewpoint -->

    <owl:Class rdf:about="http://www.semanticweb.org/activage/ontologies/2018/4/activage-core#DeltaDewpoint">
        <rdfs:subClassOf rdf:resource="http://www.semanticweb.org/activage/ontologies/2018/4/activage-core#DewCell"/>
        <rdfs:comment xml:lang="en">Device that measures the difference between Dewpoint and surface temperatures.</rdfs:comment>
        <rdfs:label xml:lang="en">Delta Dew Point</rdfs:label>
    </owl:Class>
    


    <!-- http://www.semanticweb.org/activage/ontologies/2018/4/activage-core#DewCell -->

    <owl:Class rdf:about="http://www.semanticweb.org/activage/ontologies/2018/4/activage-core#DewCell">
        <rdfs:subClassOf rdf:resource="http://www.semanticweb.org/activage/ontologies/2018/4/activage-core#HumiditySensor"/>
        <rdfs:subClassOf>
            <owl:Restriction>
                <owl:onProperty rdf:resource="http://inter-iot.eu/GOIoTP#hasUnit"/>
                <owl:someValuesFrom rdf:resource="http://sweet.jpl.nasa.gov/2.3/reprSciUnits.owl#BaseUnit"/>
            </owl:Restriction>
        </rdfs:subClassOf>
        <rdfs:subClassOf>
            <owl:Restriction>
                <owl:onProperty rdf:resource="http://www.w3.org/ns/sosa/observes"/>
                <owl:someValuesFrom rdf:resource="http://www.semanticweb.org/activage/ontologies/2018/4/activage-core#DewPoint"/>
            </owl:Restriction>
        </rdfs:subClassOf>
        <rdfs:comment>A Dew Cell is an instrument used for determining the dew point. A dew cell heats a salt solution until its equilibrium vapour pressure equals to the ambient vapour pressure, and maintains this equilibrium The temperature when this occurs is measured and it provides a measure of the ambient vapour pressure</rdfs:comment>
        <rdfs:label>Dew Cell</rdfs:label>
        <rdfs:seeAlso>http://www.hydrometeoindustry.org/Meetings2010/ET-AWS-6/Doc8[1]-AWS-MetadataCatalogues.pdf</rdfs:seeAlso>
    </owl:Class>
    


    <!-- http://www.semanticweb.org/activage/ontologies/2018/4/activage-core#DewPoint -->

    <owl:Class rdf:about="http://www.semanticweb.org/activage/ontologies/2018/4/activage-core#DewPoint">
        <rdfs:subClassOf rdf:resource="http://inter-iot.eu/GOIoTPex#Temperature"/>
        <rdfs:comment>The dew point is the temperature to which air must be cooled to become saturated with water vapor.</rdfs:comment>
        <rdfs:seeAlso>https://en.wikipedia.org/wiki/Dew_point</rdfs:seeAlso>
    </owl:Class>
    


    <!-- http://www.semanticweb.org/activage/ontologies/2018/4/activage-core#ElectricitySensor -->

    <owl:Class rdf:about="http://www.semanticweb.org/activage/ontologies/2018/4/activage-core#ElectricitySensor">
        <rdfs:subClassOf rdf:resource="http://www.w3.org/ns/sosa/Sensor"/>
        <rdfs:comment xml:lang="en">The Electricity sensor detects and measures the active power current along an electrical wire using the magnetic field with the watt.</rdfs:comment>
        <rdfs:label xml:lang="en">Electricity Sensor</rdfs:label>
    </owl:Class>
    


    <!-- http://www.semanticweb.org/activage/ontologies/2018/4/activage-core#Health -->

    <owl:Class rdf:about="http://www.semanticweb.org/activage/ontologies/2018/4/activage-core#Health">
        <rdfs:subClassOf rdf:resource="http://inter-iot.eu/GOIoTP#DomainOfInterest"/>
        <rdfs:comment xml:lang="en">Health care as an Internet of Things (IoT) applicative domain.</rdfs:comment>
        <rdfs:label xml:lang="en">Health Care DOI</rdfs:label>
    </owl:Class>
    


    <!-- http://www.semanticweb.org/activage/ontologies/2018/4/activage-core#HumiditySensor -->

    <owl:Class rdf:about="http://www.semanticweb.org/activage/ontologies/2018/4/activage-core#HumiditySensor">
        <rdfs:subClassOf rdf:resource="http://www.w3.org/ns/sosa/Sensor"/>
        <rdfs:label>Humidity Sensor</rdfs:label>
    </owl:Class>
    


    <!-- http://www.semanticweb.org/activage/ontologies/2018/4/activage-core#IlluminanceSensor -->

    <owl:Class rdf:about="http://www.semanticweb.org/activage/ontologies/2018/4/activage-core#IlluminanceSensor">
        <rdfs:subClassOf rdf:resource="http://www.w3.org/ns/sosa/Sensor"/>
        <rdfs:subClassOf>
            <owl:Restriction>
                <owl:onProperty rdf:resource="http://www.w3.org/ns/sosa/observes"/>
                <owl:someValuesFrom rdf:resource="http://inter-iot.eu/GOIoTPex#Illuminance"/>
            </owl:Restriction>
        </rdfs:subClassOf>
    </owl:Class>
    


    <!-- http://www.semanticweb.org/activage/ontologies/2018/4/activage-core#OfficeCO2Sensor -->

    <owl:Class rdf:about="http://www.semanticweb.org/activage/ontologies/2018/4/activage-core#OfficeCO2Sensor">
        <rdfs:subClassOf rdf:resource="http://www.w3.org/ns/sosa/Sensor"/>
        <rdfs:comment xml:lang="en">Carbon Dioxide (CO2) Sensor used to measure level of CO2 in the atmosphere of the office.</rdfs:comment>
        <rdfs:label xml:lang="en">Office CO2 Sensor</rdfs:label>
    </owl:Class>
    


    <!-- http://www.semanticweb.org/activage/ontologies/2018/4/activage-core#OfficeHumiditySensor -->

    <owl:Class rdf:about="http://www.semanticweb.org/activage/ontologies/2018/4/activage-core#OfficeHumiditySensor">
        <rdfs:subClassOf rdf:resource="http://www.semanticweb.org/activage/ontologies/2018/4/activage-core#HumiditySensor"/>
        <rdfs:comment xml:lang="en">Humidity sensor or hygrometer is an instrument used for measuring the moisture concent in the environment.</rdfs:comment>
        <rdfs:label xml:lang="en">Office Humidity Sensor</rdfs:label>
    </owl:Class>
    


    <!-- http://www.semanticweb.org/activage/ontologies/2018/4/activage-core#OfficeIlluminationSensor -->

    <owl:Class rdf:about="http://www.semanticweb.org/activage/ontologies/2018/4/activage-core#OfficeIlluminationSensor">
        <rdfs:subClassOf rdf:resource="http://www.semanticweb.org/activage/ontologies/2018/4/activage-core#IlluminanceSensor"/>
        <rdfs:label xml:lang="en">Office Illumination Sensor</rdfs:label>
    </owl:Class>
    


    <!-- http://www.semanticweb.org/activage/ontologies/2018/4/activage-core#OfficeTemperatureSensor -->

    <owl:Class rdf:about="http://www.semanticweb.org/activage/ontologies/2018/4/activage-core#OfficeTemperatureSensor">
        <rdfs:subClassOf rdf:resource="http://www.semanticweb.org/activage/ontologies/2018/4/activage-core#TemperatureSensor"/>
        <rdfs:comment xml:lang="en">The temperature of the air in the office that would be indicated by a thermometer exposed to the air at a location sheltered from direct solar radiation.</rdfs:comment>
        <rdfs:label xml:lang="en">Office Temperature Sensor</rdfs:label>
    </owl:Class>
    


    <!-- http://www.semanticweb.org/activage/ontologies/2018/4/activage-core#OutputVoltageSensor -->

    <owl:Class rdf:about="http://www.semanticweb.org/activage/ontologies/2018/4/activage-core#OutputVoltageSensor">
        <rdfs:subClassOf rdf:resource="http://www.w3.org/ns/sosa/Sensor"/>
        <rdfs:comment xml:lang="en">Device which can measure the difference in electric potential energy between two points per unit electric charge.</rdfs:comment>
        <rdfs:label xml:lang="en">Output Voltage Sensor</rdfs:label>
    </owl:Class>
    


    <!-- http://www.semanticweb.org/activage/ontologies/2018/4/activage-core#ParkingSensor -->

    <owl:Class rdf:about="http://www.semanticweb.org/activage/ontologies/2018/4/activage-core#ParkingSensor">
        <rdfs:subClassOf rdf:resource="http://www.w3.org/ns/sosa/Sensor"/>
        <rdfs:comment xml:lang="en">Parking sensor is proximity sensor for road vehicles designed to alert the driver of obstacles while parking</rdfs:comment>
        <rdfs:label xml:lang="en">Parking Sensor</rdfs:label>
    </owl:Class>
    


    <!-- http://www.semanticweb.org/activage/ontologies/2018/4/activage-core#Presence -->

    <owl:Class rdf:about="http://www.semanticweb.org/activage/ontologies/2018/4/activage-core#Presence">
        <rdfs:subClassOf rdf:resource="http://www.w3.org/ns/sosa/ObservableProperty"/>
    </owl:Class>
    


    <!-- http://www.semanticweb.org/activage/ontologies/2018/4/activage-core#PresenceObs -->

    <owl:Class rdf:about="http://www.semanticweb.org/activage/ontologies/2018/4/activage-core#PresenceObs">
        <rdfs:subClassOf rdf:resource="http://www.w3.org/ns/sosa/Observation"/>
        <rdfs:subClassOf>
            <owl:Restriction>
                <owl:onProperty rdf:resource="http://inter-iot.eu/GOIoTP#hasResultValue"/>
                <owl:someValuesFrom rdf:resource="http://www.w3.org/2001/XMLSchema#boolean"/>
            </owl:Restriction>
        </rdfs:subClassOf>
        <rdfs:label xml:lang="en">Presence Observation</rdfs:label>
    </owl:Class>
    


    <!-- http://www.semanticweb.org/activage/ontologies/2018/4/activage-core#RadiationSensor -->

    <owl:Class rdf:about="http://www.semanticweb.org/activage/ontologies/2018/4/activage-core#RadiationSensor">
        <rdfs:subClassOf rdf:resource="http://www.w3.org/ns/sosa/Sensor"/>
        <rdfs:comment xml:lang="en">A radiation sensor was a type of sensor that measured radiation</rdfs:comment>
        <rdfs:label xml:lang="en">Radiation Sensor</rdfs:label>
    </owl:Class>
    


    <!-- http://www.semanticweb.org/activage/ontologies/2018/4/activage-core#RelativeHumiditySensor -->

    <owl:Class rdf:about="http://www.semanticweb.org/activage/ontologies/2018/4/activage-core#RelativeHumiditySensor">
        <rdfs:subClassOf rdf:resource="http://www.semanticweb.org/activage/ontologies/2018/4/activage-core#HumiditySensor"/>
        <rdfs:comment xml:lang="en">Certain materials interact with water vapour and undergo a change in 
electrical resistance, in relation to ambient humidity.</rdfs:comment>
        <rdfs:label xml:lang="en">Relative Humidity Sensor</rdfs:label>
    </owl:Class>
    


    <!-- http://www.semanticweb.org/activage/ontologies/2018/4/activage-core#SoundLevelSensor -->

    <owl:Class rdf:about="http://www.semanticweb.org/activage/ontologies/2018/4/activage-core#SoundLevelSensor">
        <rdfs:subClassOf rdf:resource="http://www.w3.org/ns/sosa/Sensor"/>
        <rdfs:comment xml:lang="en">A sound level sensor is used to detect Noise level.</rdfs:comment>
        <rdfs:label xml:lang="en">Sound Level Sensor</rdfs:label>
    </owl:Class>
    


    <!-- http://www.semanticweb.org/activage/ontologies/2018/4/activage-core#TemperatureSensor -->

    <owl:Class rdf:about="http://www.semanticweb.org/activage/ontologies/2018/4/activage-core#TemperatureSensor">
        <rdfs:subClassOf rdf:resource="http://www.w3.org/ns/sosa/Sensor"/>
        <rdfs:label xml:lang="en">Temperature Sensor</rdfs:label>
    </owl:Class>
    


    <!-- http://www.semanticweb.org/activage/ontologies/2018/4/activage-core#Transportation -->

    <owl:Class rdf:about="http://www.semanticweb.org/activage/ontologies/2018/4/activage-core#Transportation">
        <rdfs:subClassOf rdf:resource="http://inter-iot.eu/GOIoTP#DomainOfInterest"/>
        <rdfs:comment xml:lang="en">Transportation, Smart Car/Vehicle, Intelligent Transport System (ITS) as an Internet of Things (IoT) applicative domain.</rdfs:comment>
        <rdfs:label xml:lang="en">Transportation DOI</rdfs:label>
    </owl:Class>
    


    <!-- http://www.semanticweb.org/activage/ontologies/2018/4/activage-core#UserOccupancySensor -->

    <owl:Class rdf:about="http://www.semanticweb.org/activage/ontologies/2018/4/activage-core#UserOccupancySensor">
        <rdfs:subClassOf rdf:resource="http://www.w3.org/ns/sosa/Sensor"/>
        <rdfs:subClassOf>
            <owl:Restriction>
                <owl:onProperty rdf:resource="http://www.w3.org/ns/sosa/madeObservation"/>
                <owl:someValuesFrom rdf:resource="http://www.semanticweb.org/activage/ontologies/2018/4/activage-core#PresenceObs"/>
            </owl:Restriction>
        </rdfs:subClassOf>
        <rdfs:comment xml:lang="en">The User Occupancy Sensor is an indoor motion detecting devices used to detect the presence of a person to automatically control lights or temperature or ventilation systems</rdfs:comment>
        <rdfs:label xml:lang="en">User Occupancy Sensor</rdfs:label>
    </owl:Class>
    


    <!-- http://www.semanticweb.org/activage/ontologies/2018/4/activage-core#UserPresenceSensor -->

    <owl:Class rdf:about="http://www.semanticweb.org/activage/ontologies/2018/4/activage-core#UserPresenceSensor">
        <rdfs:subClassOf rdf:resource="http://www.w3.org/ns/sosa/Sensor"/>
        <rdfs:subClassOf>
            <owl:Restriction>
                <owl:onProperty rdf:resource="http://www.w3.org/ns/sosa/madeObservation"/>
                <owl:someValuesFrom rdf:resource="http://www.semanticweb.org/activage/ontologies/2018/4/activage-core#PresenceObs"/>
            </owl:Restriction>
        </rdfs:subClassOf>
        <rdfs:comment xml:lang="en">Device used to detect if an object (vehicle, room, place, etc.) is occupied by User</rdfs:comment>
        <rdfs:label xml:lang="en">User Presence Sensor</rdfs:label>
    </owl:Class>
    


    <!-- http://www.w3.org/ns/sosa/Observation -->

    <rdf:Description rdf:about="http://www.w3.org/ns/sosa/Observation">
        <rdfs:subClassOf rdf:resource="http://www.w3.org/ns/ssn/Output"/>
    </rdf:Description>
    


    <!-- 
    ///////////////////////////////////////////////////////////////////////////////////////
    //
    // Individuals
    //
    ///////////////////////////////////////////////////////////////////////////////////////
     -->

    


    <!-- http://www.semanticweb.org/activage/ontologies/2018/4/activage-core#Index -->

    <owl:NamedIndividual rdf:about="http://www.semanticweb.org/activage/ontologies/2018/4/activage-core#Index"/>
</rdf:RDF>



<!-- Generated by the OWL API (version 4.2.8.20170104-2310) https://github.com/owlcs/owlapi -->

